language_formalisation/type_system/bidirectional.v
@@ -1,83 +1,83 @@
 Add LoadPath "C:\Users\Ziga\Documents\Ziga_podatki\PHD\language_formalisation\syntax".
 Require Import syntax.
 
-Inductive vtysynth : ctx -> val -> vtype -> Type :=
-| SynthUnit Γ : vtysynth Γ Unit TyUnit 
-| SynthInt Γ n : vtysynth Γ (Int n) TyInt
+Inductive vsynth : ctx -> val -> vtype -> Type :=
+| SynthUnit Γ : vsynth Γ Unit TyUnit 
+| SynthInt Γ n : vsynth Γ (Int n) TyInt
 | SynthVar Γ id α :
     get_vtype Γ id = Some α ->
-    vtysynth Γ (Var id) α
+    vsynth Γ (Var id) α
 | SynthPair Γ v1 v2 α β :
-    vtysynth Γ v1 α ->
-    vtysynth Γ v2 β ->
-    vtysynth Γ (Pair v1 v2) (TyΠ α β)
+    vsynth Γ v1 α ->
+    vsynth Γ v2 β ->
+    vsynth Γ (Pair v1 v2) (TyΠ α β)
 | SynthVAnnot Γ v α :
-    vtycheck Γ v α ->
-    vtysynth Γ (VAnnot v α) α
-with ctysynth : ctx -> comp -> ctype -> Type :=
-| SynthRet Γ v α : ctysynth Γ (Ret v) (CTy α SigØ EqsØ)
+    vcheck Γ v α ->
+    vsynth Γ (VAnnot v α) α
+with csynth : ctx -> comp -> ctype -> Type :=
+| SynthRet Γ v α : csynth Γ (Ret v) (CTy α SigØ EqsØ)
 | SynthPMatch Γ v α β x y c ctyC :
-    vtysynth Γ v (TyΠ α β) ->
-    ctysynth (CtxU x α (CtxU y β Γ)) c ctyC ->
-    ctysynth Γ c ctyC
+    vsynth Γ v (TyΠ α β) ->
+    csynth (CtxU x α (CtxU y β Γ)) c ctyC ->
+    csynth Γ c ctyC
 | SynthApp Γ v1 v2 α ctyC :
-    vtysynth Γ v1 (TyFun α ctyC) ->
-    vtycheck Γ v2 α ->
-    ctysynth Γ (App v1 v2) ctyC
+    vsynth Γ v1 (TyFun α ctyC) ->
+    vcheck Γ v2 α ->
+    csynth Γ (App v1 v2) ctyC
 | SynthHandle Γ v c ctyC ctyD :
-    vtysynth Γ v (TyHandler ctyC ctyD) ->
-    ctycheck Γ c ctyC ->
-    ctysynth Γ (Handle v c) ctyC
+    vsynth Γ v (TyHandler ctyC ctyD) ->
+    ccheck Γ c ctyC ->
+    csynth Γ (Handle v c) ctyC
 | SynthCAnnot Γ c ctyC :
-    ctycheck Γ c ctyC ->
-    ctysynth Γ (CAnnot c ctyC) ctyC
-(* with htysynth : ctx -> hcases -> sig -> ctype -> Type := *)
-with vtycheck : ctx -> val -> vtype -> Type :=
+    ccheck Γ c ctyC ->
+    csynth Γ (CAnnot c ctyC) ctyC
+(* with hsynth : ctx -> hcases -> sig -> ctype -> Type := *)
+with vcheck : ctx -> val -> vtype -> Type :=
 | CheckVBySynth Γ v α α' :
-    vtysynth Γ v α' ->
+    vsynth Γ v α' ->
     α = α' ->
-    vtycheck Γ v α
+    vcheck Γ v α
 | CheckInl Γ v α β :
-    vtycheck Γ v α ->
-    vtycheck Γ (Inl v) (TyΣ α β)
+    vcheck Γ v α ->
+    vcheck Γ (Inl v) (TyΣ α β)
 | CheckInr Γ v α β :
-    vtycheck Γ v β ->
-    vtycheck Γ (Inr v) (TyΣ α β)
+    vcheck Γ v β ->
+    vcheck Γ (Inr v) (TyΣ α β)
 | CheckPair Γ v1 v2 α β :
-    vtycheck Γ v1 α ->
-    vtycheck Γ v2 β ->
-    vtycheck Γ (Pair v1 v2) (TyΠ α β)
+    vcheck Γ v1 α ->
+    vcheck Γ v2 β ->
+    vcheck Γ (Pair v1 v2) (TyΠ α β)
 | CheckFun Γ x c α tyC :
-    ctycheck (CtxU x α Γ) c tyC ->
-    vtycheck Γ (Fun x c) (TyFun α tyC)
+    ccheck (CtxU x α Γ) c tyC ->
+    vcheck Γ (Fun x c) (TyFun α tyC)
 | CheckHandler Γ x c_ret h α sig eqs ctyD :
-    ctycheck (CtxU x α Γ) c_ret ctyD ->
-    htycheck Γ h sig ctyD ->
-    vtycheck Γ (Handler x c_ret h) (TyHandler (CTy α sig eqs) ctyD)
-with ctycheck : ctx -> comp -> ctype -> Type :=
+    ccheck (CtxU x α Γ) c_ret ctyD ->
+    hcheck Γ h sig ctyD ->
+    vcheck Γ (Handler x c_ret h) (TyHandler (CTy α sig eqs) ctyD)
+with ccheck : ctx -> comp -> ctype -> Type :=
 | CheckCBySynth Γ c ctyC ctyC' :
-    ctysynth Γ c ctyC' ->
+    csynth Γ c ctyC' ->
     ctyC = ctyC' ->
-    ctycheck Γ c ctyC
+    ccheck Γ c ctyC
 | CheckSMatch Γ v α β xl cl xr cr ctyC :
-    vtysynth Γ v (TyΣ α β) ->
-    ctycheck (CtxU xl α Γ) cl ctyC ->
-    ctycheck (CtxU xr β Γ) cr ctyC ->
-    ctycheck Γ (ΣMatch v xl cl xr cr) ctyC
+    vsynth Γ v (TyΣ α β) ->
+    ccheck (CtxU xl α Γ) cl ctyC ->
+    ccheck (CtxU xr β Γ) cr ctyC ->
+    ccheck Γ (ΣMatch v xl cl xr cr) ctyC
 | CheckOp Γ op_id v y c α_op β_op α sig eqs :
     get_op_type sig op_id = Some (α_op, β_op) ->
-    vtycheck Γ v α_op ->
-    ctycheck (CtxU y β_op Γ) c (CTy α sig eqs) ->
-    ctycheck Γ (Op op_id v y c) (CTy α sig eqs)
-with htycheck : ctx -> hcases -> sig -> ctype -> Type :=
-| CheckCasesØ Γ ctyD : htycheck Γ CasesØ SigØ ctyD
+    vcheck Γ v α_op ->
+    ccheck (CtxU y β_op Γ) c (CTy α sig eqs) ->
+    ccheck Γ (Op op_id v y c) (CTy α sig eqs)
+with hcheck : ctx -> hcases -> sig -> ctype -> Type :=
+| CheckCasesØ Γ ctyD : hcheck Γ CasesØ SigØ ctyD
 | CheckCasesU Γ h op_id x k c_op α_op β_op sig ctyD :
     find_op_case h op_id = None ->
-    htycheck Γ h sig ctyD ->
-    ctycheck
+    hcheck Γ h sig ctyD ->
+    ccheck
       (CtxU x α_op (CtxU k (TyFun β_op ctyD) Γ))
       c_op ctyD ->
-    htycheck 
+    hcheck 
       Γ (CasesU h op_id x k c_op)
       (SigU op_id α_op β_op sig) ctyD
 .
