language_formalisation/type_system/lemmas.v
@@ -1,0 +1,44 @@
+Add LoadPath "C:\Users\Ziga\Documents\Ziga_podatki\PHD\language_formalisation\syntax".
+Add LoadPath "C:\Users\Ziga\Documents\Ziga_podatki\PHD\language_formalisation\type_system".
+Require Export syntax bidirectional Omega Logic.
+
+Ltac inv H := inversion H; clear H; subst.
+
+
+Lemma val_emptyctx_substitution_lemma
+  (prog : val) (A : vtype)
+  (x : var_id) (v : val) (α : vtype) :
+  vcheck (CtxU x α CtxØ) prog A ->
+  vcheck CtxØ v α ->
+  vcheck CtxØ (vsubst (x, v) prog) A.
+Proof.
+  revert A.
+  induction prog; intros A typed_original typed_v.
+  - induction (s == x). simpl.
+    + inv typed_original. inv H. simpl in H2.
+      induction (x == x).
+      * inv H2.
+        assumption.
+      * destruct b.
+        reflexivity.
+    + inv typed_original. inv H. simpl in H2.
+      destruct (s==x) in H2.
+      * destruct b. exact e.
+      * discriminate.
+  - inv typed_original. inv H.
+    exact (CheckVBySynth CtxØ Unit _ _ (SynthUnit CtxØ) (eq_refl _)).
+  - inv typed_original. inv H.
+    exact (CheckVBySynth CtxØ (Int t) _ _ (SynthInt CtxØ t) (eq_refl _)).
+  - simpl. inv typed_original.
+    + inv H.
+    + apply IHprog in H1.
+      exact (CheckInl CtxØ _ α0 β H1).
+      assumption.
+  - simpl. inv typed_original.
+    + inv H.
+    + apply IHprog in H1.
+      exact (CheckInr CtxØ _ α0 β H1).
+      assumption.
+  - 
+      
+Qed.
